F8 abbrev and appropriate conversion lemmas.

Clap/eDSLState/Convert/Specialised.lean
@@ -12,6 +12,7 @@ section User
 
 abbrev F (p : ℕ) : Type := HashConsM.BoundRef p
 abbrev FB (p : ℕ) : Type := F p
+abbrev F8 (p : ℕ) : Type := F p
 abbrev FArray (p k : ℕ) : Type := Vector (FB p) k
 abbrev FList (p : ℕ) : Type := List (FB p)
 
@@ -66,6 +67,14 @@ abbrev conversion : Conversion p (FB p) where
 
 end FB
 
+namespace F8
+
+abbrev conversion : Conversion p (F8 p) where
+  IdealT := UInt8
+  toExprs x := [x]
+  conversion x := [(x.toNat : ZMod p)]
+
+end F8
 
 namespace FUnit
 
@@ -117,12 +126,26 @@ lemma converts_of_FB_converts
   (val2 := if b then (1 : ZMod p) else (0 : ZMod p))
   h (by rfl) (by rfl)
 
+lemma converts_of_F8_converts
+  {state : ClapMState p}
+  {expr : F8 p}
+  {u : UInt8}
+  (h : Converts F8.conversion state expr u)
+:
+  Converts F.conversion state expr (u.toNat : ZMod p)
+:= converts_cast
+  (conversion1 := F8.conversion)
+  (conversion2 := F.conversion)
+  (y := expr)
+  (val2 := (u.toNat : ZMod p))
+  h (by rfl) (by rfl)
+
 end F
 
 namespace FB
 
 lemma converts_of_F_converts
-  [p.AtLeastTwo]
+  [NeZero p]
   {state : ClapMState p}
   {expr : F p}
   {val}
@@ -138,13 +161,18 @@ lemma converts_of_F_converts
     split
     . trivial
     next h_neq =>
-      rewrite [←ZMod.val_eq_zero]
-      rewrite [←ZMod.val_eq_one] at h_neq
-      grind
-      exact Nat.AtLeastTwo.one_lt
+      have h_ne : val ≠ 1 := by simpa using h_neq
+      have h01 : val.val = 0 ∨ val.val = 1 := by omega
+      rcases h01 with h0 | h1
+      . exact (ZMod.val_eq_zero val).mp h0
+      . exfalso
+        apply h_ne
+        have h_round := ZMod.natCast_rightInverse (n := p) val
+        rw [h1] at h_round
+        simpa using h_round.symm
 
 lemma convertsM_of_F_convertsM
-  [p.AtLeastTwo]
+  [NeZero p]
   {action : ClapM p (F p)}
   {state : ClapMState p}
   {val : ZMod p}
@@ -161,6 +189,42 @@ lemma convertsM_of_F_convertsM
 
 end FB
 
+namespace F8
+
+lemma converts_of_F_converts
+  [NeZero p]
+  {state : ClapMState p}
+  {expr : F p}
+  {val}
+  (h : Converts F.conversion state expr val)
+  (h_val : val.val < UInt8.size)
+:
+  Converts F8.conversion state (expr : F8 p) (UInt8.ofNat val.val)
+:= by
+  apply converts_cast h
+  . rfl
+  . unfold F.conversion conversion
+    simp
+    rw [Nat.mod_eq_of_lt h_val]
+    exact (ZMod.natCast_rightInverse (n := p) val).symm
+
+lemma convertsM_of_F_convertsM
+  [NeZero p]
+  {action : ClapM p (F p)}
+  {state : ClapMState p}
+  {val : ZMod p}
+  {constraints}
+  (h : ConvertsM F.conversion action state val constraints)
+  (h_val : val.val < UInt8.size)
+:
+  ConvertsM F8.conversion action state (UInt8.ofNat val.val) constraints
+:= by
+  constructor
+  . exact converts_of_F_converts h.result h_val
+  . exact h.wellFormed
+  . exact h.constraints
+
+end F8
 
 namespace FUnit
 
